updated schedule_oracle to have two sublocales  and  for its two use cases (our old locale and new nlds stuff). new lemmas in there, and updated timeprotection integration to use the new  locale, which gives us the properties we need.
Signed-off-by: Scott Buckley <s.buckley@unsw.edu.au>

proof/infoflow/timeprotection/TimeProtectionIntegration.thy
@@ -20,8 +20,11 @@ locale integration_setup =
   for gentypes :: "('fch \<times> 'fch_cachedness \<times> 'pch \<times> 'pch_cachedness \<times> 'l partition \<times> 'colour) itself"
   and initial_aag :: "'l subject_label PAS"
 + fixes time_per_tick :: time
-  fixes fixme_WCET :: time
+  fixes slice_length_min :: time
+  fixes timer_delay_max :: time
   fixes ta :: "if_other_state \<Rightarrow> vpaddr set"
+  assumes timer_delay_lt_slice_length:
+    "timer_delay_max < slice_length_min"
 begin
 
 (* get the list of (domain, tickcount) from the initial state *)
@@ -34,26 +37,28 @@ definition dom_list_internal where
 definition schedule_list where
   "schedule_list \<equiv> map (\<lambda>(d, ticks). (data_to_nat ticks * time_per_tick, d)) dom_list_internal"
 
-interpretation sched_o:schedule_oracle _ schedule_list fixme_WCET
+interpretation sched_o:schedule_oracle_delayed _ schedule_list slice_length_min timer_delay_max
   apply unfold_locales
    (* we need to know that the domain list has some minimum time *)
    subgoal sorry
   (* we need to know that the domain list is never empty *)
   subgoal sorry
+
+  subgoal sorry
   done
 
 definition nlds where
-  "nlds \<equiv> sched_o.slice_end"
+  "nlds \<equiv> sched_o.next_delayed_start"
 
 lemma nlds_in_future:
-  "t \<le> nlds t"
-  apply (clarsimp simp:nlds_def)
-  apply (simp add: le_simps(1) sched_o.slice_end_gt)
+  "t < nlds t"
+  apply (clarsimp simp:nlds_def sched_o.next_delayed_start_in_future)
   done
 
-lemma nlds_step:
-  "\<lbrakk>t \<le> t'; t' \<le> nlds t\<rbrakk> \<Longrightarrow> nlds t' = nlds t"
-  sledgehammer
+lemma nlds_flatsteps:
+  "\<lbrakk>t \<le> t'; t' < nlds t\<rbrakk> \<Longrightarrow> nlds t' = nlds t"
+  apply (clarsimp simp:nlds_def sched_o.next_delayed_start_flatsteps)
+  done
                     
 interpretation tphuwr:time_protection_hardware_uwr gentypes PSched 
   _ _ _ _ _ _ _ _ _ _ _ _ _ _ _ _ _ _ part uwr nlds ta
@@ -107,7 +112,7 @@ pch_read_impact :: "paddr \<Rightarrow> 'pch \<Rightarrow> 'pch"
     and addr_colour :: "paddr \<Rightarrow> 'colour"
     and colour_userdomain :: "'colour \<Rightarrow> 'domain"
  *)
-
+thm in_opt_map_eq
 interpretation ma?:time_protection_system PSched fch_lookup fch_read_impact fch_write_impact
   empty_fch fch_flush_cycles fch_flush_WCET pch_lookup pch_read_impact pch_write_impact do_pch_flush
   pch_flush_cycles pch_flush_WCET collides_in_pch read_cycles write_cycles addr_domain addr_colour colour_userdomain
@@ -119,7 +124,7 @@ interpretation ma?:time_protection_system PSched fch_lookup fch_read_impact fch_
               apply (simp add: uwr_equiv_rel)
              subgoal sorry
             apply (rule nlds_in_future)
-           subgoal sorry
+           apply (rule nlds_flatsteps; simp)
           subgoal sorry
          subgoal sorry
         subgoal sorry
